Update goose output for unit tests and goose-nfsd

src/goose_lang/examples/goose_semantics.v
@@ -854,7 +854,7 @@ Definition testArithmeticShifts: val :=
     "ok" <-[boolT] (![boolT] "ok") && (#672 ≪ #51 = #1513209474796486656);;
     "ok" <-[boolT] (![boolT] "ok") && (#672 ≫ #4 = #42);;
     "ok" <-[boolT] (![boolT] "ok") && (#672 ≫ #12 = #0);;
-    "ok" <-[boolT] (![boolT] "ok") && (#672 ≫ #4 ≪ #4 = #672);;
+    "ok" <-[boolT] (![boolT] "ok") && ((#672 ≫ #4) ≪ #4 = #672);;
     ![boolT] "ok".
 
 (* precedence.go *)
@@ -890,6 +890,10 @@ Definition testAndCompare: val :=
     then #()
     else "ok" <-[boolT] #false);;
     ![boolT] "ok".
+
+Definition testShiftMod: val :=
+  rec: "testShiftMod" <> :=
+    (#20 ≫ (#8 `rem` #4) = #20).
 
 (* prims.go *)
 
