external/Goose/github_com/mit_pdos/goose_nfsd/twophase.v
@@ -99,14 +99,14 @@ Definition TwoPhase__OverWrite: val :=
 Definition TwoPhase__ReadBufBit: val :=
   rec: "TwoPhase__ReadBufBit" "twophase" "addr" :=
     let: "dataByte" := SliceGet byteT (TwoPhase__ReadBuf "twophase" "addr" #1) #0 in
-    ("dataByte" ≫ (struct.get addr.Addr.S "Off" "addr") `rem` #8 = #(U8 1)).
+    ("dataByte" ≫ ((struct.get addr.Addr.S "Off" "addr") `rem` #8) = #(U8 1)).
 
 Definition TwoPhase__OverWriteBit: val :=
   rec: "TwoPhase__OverWriteBit" "twophase" "addr" "data" :=
     let: "dataByte" := ref (zero_val byteT) in
     (if: "data"
     then
-      "dataByte" <-[byteT] #(U8 1) ≪ (struct.get addr.Addr.S "Off" "addr") `rem` #8;;
+      "dataByte" <-[byteT] (#(U8 1)) ≪ ((struct.get addr.Addr.S "Off" "addr") `rem` #8);;
       #()
     else #());;
     TwoPhase__OverWrite "twophase" "addr" #1 (SliceSingleton (![byteT] "dataByte")).
